Weidenbach_Book/IsaSAT_Trail.thy
@@ -7,6 +7,9 @@ lemma list_rel_take:
   \<open>(ba, ab) \<in> \<langle>A\<rangle>list_rel \<Longrightarrow> (take b ba, take b ab) \<in> \<langle>A\<rangle>list_rel\<close>
   by (auto simp: list_rel_def)
 
+text \<open>
+  This function does not resize the array: this makes sense for our purpose, but may be not in
+  general.\<close>
 definition butlast_arl where
   \<open>butlast_arl = (\<lambda>(xs, i). (xs, fast_minus i 1))\<close>
 
@@ -147,6 +150,16 @@ lemma array_option_uint32_of_nat_conv_hnr[sepref_fr_rules]:
   using array_option_uint32_of_nat_code.refine[unfolded array_option_uint32_of_nat_def,
     FCOMP op_map_map_rel] unfolding array_option_uint32_of_nat_conv_alt_def
   by simp
+
+definition nat_of_uint32_spec :: \<open>nat \<Rightarrow> nat\<close> where
+  [simp]: \<open>nat_of_uint32_spec n = n\<close>
+
+lemma nat_of_uint32_spec_hnr[sepref_fr_rules]:
+  \<open>(return o uint32_of_nat, RETURN o nat_of_uint32_spec) \<in>
+     [\<lambda>n. n \<le> uint32_max]\<^sub>a nat_assn\<^sup>k \<rightarrow> uint32_nat_assn\<close>
+  by sepref_to_hoare
+    (sep_auto simp: uint32_nat_rel_def br_def nat_of_uint32_spec_def
+      nat_of_uint32_uint32_of_nat_id)
 (* End Move *)
 
 type_synonym tri_bool = \<open>bool option\<close>
@@ -219,13 +232,15 @@ lemma [safe_constraint_rules]:
   by auto
 
 type_synonym trail_pol =
-   \<open>nat literal list \<times> tri_bool list \<times> nat list \<times> nat option list \<times> nat\<close>
+   \<open>nat literal list \<times> tri_bool list \<times> nat list \<times> nat option list \<times> nat \<times> nat list\<close>
 
 type_synonym trail_pol_assn =
-   \<open>uint32 array_list \<times> tri_bool_assn array \<times> uint32 array \<times> nat option array \<times> uint32\<close>
+   \<open>uint32 array_list \<times> tri_bool_assn array \<times> uint32 array \<times> nat option array \<times> uint32 \<times>
+      uint32 array_list\<close>
 
 type_synonym trail_pol_fast_assn =
-   \<open>uint32 array_list \<times> tri_bool_assn array \<times> uint32 array \<times> uint32 option array \<times> uint32\<close>
+   \<open>uint32 array_list \<times> tri_bool_assn array \<times> uint32 array \<times> uint32 option array \<times> uint32 \<times>
+      uint32 array_list\<close>
 
 definition get_level_atm where
   \<open>get_level_atm M L = get_level M (Pos L)\<close>
@@ -242,6 +257,194 @@ definition defined_atm :: \<open>('v, nat) ann_lits \<Rightarrow> 'v \<Rightarro
 abbreviation undefined_atm where
   \<open>undefined_atm M L \<equiv> \<not>defined_atm M L\<close>
 
+inductive control_stack where
+empty:
+  \<open>control_stack [] []\<close> |
+cons_prop:
+  \<open>control_stack cs M \<Longrightarrow> control_stack cs (Propagated L C # M)\<close> |
+cons_dec:
+  \<open>control_stack cs M \<Longrightarrow> n = length M \<Longrightarrow> control_stack (cs @ [n]) (Decided L # M)\<close>
+
+inductive_cases control_stackE: \<open>control_stack cs M\<close>
+thm control_stackE
+lemma control_stack_length_count_dec:
+  \<open>control_stack cs M \<Longrightarrow> length cs = count_decided M\<close>
+  by (induction rule: control_stack.induct) auto
+
+lemma control_stack_le_length_M:
+  \<open>control_stack cs M \<Longrightarrow> c\<in>set cs \<Longrightarrow> c < length M\<close>
+  by (induction rule: control_stack.induct) auto
+
+lemma control_stack_propa[simp]:
+  \<open>control_stack cs (Propagated x21 x22 # list) \<longleftrightarrow> control_stack cs list\<close>
+  by (auto simp: control_stack.intros elim: control_stackE)
+
+lemma control_stack_filter_map_nth:
+  \<open>control_stack cs M \<Longrightarrow> filter is_decided (rev M) = map (nth (rev M)) cs\<close>
+  apply (induction rule: control_stack.induct)
+  subgoal by auto
+  subgoal for cs M L C
+    using control_stack_le_length_M[of cs M]
+    by (auto simp: nth_append)
+  subgoal for cs M L
+    using control_stack_le_length_M[of cs M]
+    by (auto simp: nth_append)
+  done
+
+lemma control_stack_empty_cs[simp]: \<open>control_stack [] M \<longleftrightarrow> count_decided M = 0\<close>
+  by (induction M rule:ann_lit_list_induct)
+    (auto simp: control_stack.empty control_stack.cons_prop elim: control_stackE)
+
+definition control_stack' where
+  \<open>control_stack' cs M \<longleftrightarrow>
+     (length cs = count_decided M \<and>
+      (\<forall>L\<in>set M. is_decided L \<longrightarrow> (cs ! (get_level M (lit_of L) - 1) < length M \<and> 
+          rev M!(cs ! (get_level M (lit_of L) - 1)) = L)))\<close>
+
+lemma undefined_notin: \<open>undefined_lit M (lit_of x) \<Longrightarrow> x \<notin> set M\<close> for x M
+  by (metis in_lits_of_l_defined_litD insert_iff lits_of_insert mk_disjoint_insert)
+
+lemma control_stack_rev_get_lev:
+  \<open>control_stack cs M  \<Longrightarrow>
+    no_dup M \<Longrightarrow> L\<in>set M \<Longrightarrow> is_decided L \<Longrightarrow> rev M!(cs ! (get_level M (lit_of L) - 1)) = L\<close>
+  apply (induction arbitrary: L rule: control_stack.induct)
+  subgoal by auto
+  subgoal for cs M L C La
+    using control_stack_le_length_M[of cs M] control_stack_length_count_dec[of cs M]
+      count_decided_ge_get_level[of M \<open>lit_of La\<close>]
+    apply (auto simp: get_level_cons_if nth_append atm_of_eq_atm_of undefined_notin)
+    by (metis Suc_count_decided_gt_get_level Suc_less_eq Suc_pred count_decided_0_iff diff_is_0_eq
+        le_SucI le_refl neq0_conv nth_mem)
+  subgoal for cs M L
+    using control_stack_le_length_M[of cs M] control_stack_length_count_dec[of cs M]
+    apply (auto simp: nth_append  get_level_cons_if atm_of_eq_atm_of undefined_notin)
+    by (metis Suc_count_decided_gt_get_level Suc_less_eq Suc_pred count_decided_0_iff diff_is_0_eq
+        le_SucI le_refl neq0_conv)+
+  done
+
+lemma control_stack_alt_def_imp:
+  \<open>no_dup M \<Longrightarrow> (\<And>L. L \<in>set M \<Longrightarrow> is_decided L \<Longrightarrow> cs ! (get_level M (lit_of L) - 1) < length M \<and>
+        rev M!(cs ! (get_level M (lit_of L) - 1)) = L) \<Longrightarrow>
+    length cs = count_decided M \<Longrightarrow>
+    control_stack cs M\<close>
+proof (induction M arbitrary: cs rule:ann_lit_list_induct)
+  case Nil
+  then show ?case by auto
+next
+  case (Decided L M) note IH = this(1) and n_d = this(2) and dec = this(3) and length = this(4)
+  from length obtain cs' n where cs[simp]: \<open>cs = cs' @ [n]\<close>
+    using length by (cases cs rule: rev_cases) auto
+  have [simp]: \<open>rev M ! n \<in> set M \<Longrightarrow> is_decided (rev M ! n) \<Longrightarrow> count_decided M \<noteq> 0\<close>
+    by (auto simp: count_decided_0_iff)
+  have dec': \<open>L'\<in>set M \<Longrightarrow> is_decided L' \<Longrightarrow> cs' ! (get_level M (lit_of L') - 1) < length M \<and> 
+        rev M ! (cs' ! (get_level M (lit_of L') - 1)) = L'\<close> for L'
+    using dec[of L'] n_d length
+    count_decided_ge_get_level[of M \<open>lit_of L'\<close>]
+    apply (auto simp: get_level_cons_if atm_of_eq_atm_of undefined_notin
+        split: if_splits)
+    apply (auto simp: nth_append split: if_splits)
+    done
+  have le: \<open>length cs' = count_decided M\<close>
+    using length by auto
+  have [simp]: \<open>n = length M\<close>
+    using n_d dec[of \<open>Decided L\<close>] le undefined_notin[of M \<open>rev M ! n\<close>] nth_mem[of n \<open>rev M\<close>]
+    by (auto simp: nth_append split: if_splits)
+  show ?case
+    unfolding cs
+    apply (rule control_stack.cons_dec)
+    subgoal
+      apply (rule IH)
+      using n_d dec' le by auto
+    subgoal by auto
+    done
+next
+  case (Propagated L m M) note IH = this(1) and n_d = this(2) and dec = this(3) and length = this(4)
+  have [simp]: \<open>rev M ! n \<in> set M \<Longrightarrow> is_decided (rev M ! n) \<Longrightarrow> count_decided M \<noteq> 0\<close> for n
+    by (auto simp: count_decided_0_iff)
+  have dec': \<open>L'\<in>set M \<Longrightarrow> is_decided L' \<Longrightarrow> cs ! (get_level M (lit_of L') - 1) < length M \<and> 
+        rev M ! (cs ! (get_level M (lit_of L') - 1)) = L'\<close> for L'
+    using dec[of L'] n_d length
+    count_decided_ge_get_level[of M \<open>lit_of L'\<close>]
+    apply (cases L')
+    apply (auto simp: get_level_cons_if atm_of_eq_atm_of undefined_notin
+        split: if_splits)
+    apply (auto simp: nth_append split: if_splits)
+    done
+  show ?case
+    apply (rule control_stack.cons_prop)
+    apply (rule IH)
+    subgoal using n_d by auto
+    subgoal using dec' by auto
+    subgoal using length by auto
+    done
+qed
+
+lemma control_stack_alt_def: \<open>no_dup M \<Longrightarrow> control_stack' cs M \<longleftrightarrow> control_stack cs M\<close>
+  using control_stack_alt_def_imp[of M cs] control_stack_rev_get_lev[of cs M]
+    control_stack_length_count_dec[of cs M] control_stack_le_length_M[of cs M]
+  unfolding control_stack'_def apply -
+  apply (rule iffI)
+  subgoal by blast
+  subgoal
+    using count_decided_ge_get_level[of M ]
+    by (metis One_nat_def Suc_count_decided_gt_get_level Suc_less_eq Suc_pred count_decided_0_iff
+        less_imp_diff_less neq0_conv nth_mem)
+  done
+
+lemma control_stack_decomp:
+  assumes 
+    decomp: \<open>(Decided L # M1, M2) \<in> set (get_all_ann_decomposition M)\<close> and
+    cs: \<open>control_stack cs M\<close> and
+    n_d: \<open>no_dup M\<close>
+  shows \<open>control_stack (take (count_decided M1) cs) M1\<close>
+proof -
+  obtain M3 where M: \<open>M = M3 @ M2 @ Decided L # M1\<close>
+    using decomp by auto
+  define M2' where \<open>M2' = M3 @ M2\<close>
+  have M: \<open>M = M2' @ Decided L # M1\<close>
+    unfolding M M2'_def by auto
+  have n_d1: \<open>no_dup M1\<close>
+    using n_d no_dup_appendD unfolding M by auto
+  have \<open>control_stack' cs M\<close>
+    using cs
+    apply (subst (asm) control_stack_alt_def[symmetric])
+     apply (rule n_d)
+    apply assumption
+    done
+  then have
+    cs_M: \<open>length cs = count_decided M\<close> and
+    L: \<open>\<And>L. L\<in>set M \<Longrightarrow> is_decided L \<Longrightarrow>
+      cs ! (get_level M (lit_of L) - 1) < length M \<and> rev M ! (cs ! (get_level M (lit_of L) - 1)) = L\<close>
+    unfolding control_stack'_def by auto
+  have H: \<open>L' \<in> set M1 \<Longrightarrow> undefined_lit M2' (lit_of L') \<and> atm_of (lit_of L') \<noteq> atm_of L\<close>  for L'
+    using n_d unfolding M
+    by (metis atm_of_eq_atm_of defined_lit_no_dupD(1) defined_lit_uminus lit_of.simps(1)
+        no_dup_appendD no_dup_append_cons no_dup_cons undefined_notin)
+  have \<open>distinct M\<close>
+    using no_dup_imp_distinct[OF n_d] .
+  then have K: \<open>L' \<in> set M1 \<Longrightarrow> x < length M \<Longrightarrow> rev M ! x = L' \<Longrightarrow> x < length M1\<close> for x L'
+    unfolding M apply (auto simp: nth_append nth_Cons split: if_splits nat.splits)
+    by (metis length_rev less_diff_conv local.H not_less_eq nth_mem set_rev undefined_notin)
+  have I: \<open>L \<in> set M1 \<Longrightarrow> is_decided L \<Longrightarrow> get_level M1 (lit_of L) > 0\<close> for L
+    using n_d unfolding M by (auto dest!: split_list)
+  have cs': \<open>control_stack' (take (count_decided M1) cs) M1\<close>
+    unfolding control_stack'_def
+    apply (intro conjI ballI impI)
+    subgoal using cs_M unfolding M by auto
+    subgoal for L using n_d L[of L] H[of L] K[of L \<open>cs ! (get_level M1 (lit_of L) - Suc 0)\<close>]
+        count_decided_ge_get_level[of \<open>M1\<close> \<open>lit_of L\<close>] I[of L]
+      unfolding M by auto
+    subgoal for L using n_d L[of L] H[of L] K[of L \<open>cs ! (get_level M1 (lit_of L) - Suc 0)\<close>]
+        count_decided_ge_get_level[of \<open>M1\<close> \<open>lit_of L\<close>] I[of L]
+      unfolding M by auto
+    done
+  show ?thesis
+    apply (subst control_stack_alt_def[symmetric])
+     apply (rule n_d1)
+    apply (rule cs')
+    done
+qed
+
 context isasat_input_ops
 begin
 
@@ -253,12 +456,13 @@ definition ann_lits_split_reasons where
   }\<close>
 
 definition trail_pol :: \<open>(trail_pol \<times> (nat, nat) ann_lits) set\<close> where
-  \<open>trail_pol = {((M', xs, lvls, reasons, k), M). ((M', reasons), M) \<in> ann_lits_split_reasons \<and>
+  \<open>trail_pol = {((M', xs, lvls, reasons, k, cs), M). ((M', reasons), M) \<in> ann_lits_split_reasons \<and>
     no_dup M \<and>
     (\<forall>L \<in># \<L>\<^sub>a\<^sub>l\<^sub>l. nat_of_lit L < length xs \<and> xs ! (nat_of_lit L) = polarity M L) \<and>
     (\<forall>L \<in># \<L>\<^sub>a\<^sub>l\<^sub>l. atm_of L < length lvls \<and> lvls ! (atm_of L) = get_level M L) \<and>
     k = count_decided M \<and>
-    (\<forall>L\<in>set M. lit_of L \<in># \<L>\<^sub>a\<^sub>l\<^sub>l)}\<close>
+    (\<forall>L\<in>set M. lit_of L \<in># \<L>\<^sub>a\<^sub>l\<^sub>l) \<and>
+    control_stack cs M}\<close>
 
 end
 
@@ -266,14 +470,14 @@ abbreviation trail_pol_assn :: \<open>trail_pol \<Rightarrow> trail_pol_assn \<R
   \<open>trail_pol_assn \<equiv>
       arl_assn unat_lit_assn *a array_assn (tri_bool_assn) *a
       array_assn uint32_nat_assn *a
-      array_assn (option_assn nat_assn) *a uint32_nat_assn\<close>
+      array_assn (option_assn nat_assn) *a uint32_nat_assn *a arl_assn uint32_nat_assn\<close>
 
 
 abbreviation trail_pol_fast_assn :: \<open>trail_pol \<Rightarrow> trail_pol_fast_assn \<Rightarrow> assn\<close> where
   \<open>trail_pol_fast_assn \<equiv>
       arl_assn unat_lit_assn *a array_assn (tri_bool_assn) *a
       array_assn uint32_nat_assn *a
-      array_assn (option_assn uint32_nat_assn) *a uint32_nat_assn\<close>
+      array_assn (option_assn uint32_nat_assn) *a uint32_nat_assn *a arl_assn uint32_nat_assn\<close>
 
 abbreviation phase_saver_conc where
   \<open>phase_saver_conc \<equiv> array_assn bool_assn\<close>
@@ -487,7 +691,7 @@ lemmas get_level_fast_code_get_level_code[sepref_fr_rules] =
    get_level_fast_code.refine[of \<A>\<^sub>i\<^sub>n, OF isasat_input_bounded_axioms]
 
 definition (in -) count_decided_pol where
-  \<open>count_decided_pol = (\<lambda>(_, _, _, _, k). k)\<close>
+  \<open>count_decided_pol = (\<lambda>(_, _, _, _, k, _). k)\<close>
 
 lemma count_decided_trail_ref:
   \<open>(RETURN o count_decided_pol, RETURN o count_decided) \<in> trail_pol \<rightarrow>\<^sub>f \<langle>nat_rel\<rangle>nres_rel\<close>
@@ -593,9 +797,9 @@ definition cons_trail_Propagated :: \<open>nat literal \<Rightarrow> nat \<Right
   \<open>cons_trail_Propagated L C M' = Propagated L C # M'\<close>
 
 definition cons_trail_Propagated_tr :: \<open>nat literal \<Rightarrow> nat \<Rightarrow> trail_pol \<Rightarrow> trail_pol\<close> where
-  \<open>cons_trail_Propagated_tr = (\<lambda>L C (M', xs, lvls, reasons, k).
+  \<open>cons_trail_Propagated_tr = (\<lambda>L C (M', xs, lvls, reasons, k, cs).
      (M' @ [L], let xs = xs[nat_of_lit L := Some True] in xs[nat_of_lit (-L) := Some False],
-      lvls[atm_of L := k], reasons[atm_of L:= Some C], k))\<close>
+      lvls[atm_of L := k], reasons[atm_of L:= Some C], k, cs))\<close>
 
 lemma in_list_pos_neg_notD: \<open>Pos (atm_of (lit_of La)) \<notin> lits_of_l bc \<Longrightarrow>
        Neg (atm_of (lit_of La)) \<notin> lits_of_l bc \<Longrightarrow>
@@ -613,7 +817,7 @@ lemma cons_trail_Propagated_tr:
         dest!: in_list_pos_neg_notD multi_member_split dest: pos_lit_in_atms_of neg_lit_in_atms_of
          simp del: nat_of_lit.simps)
 
-lemma undefined_lit_count_decided_uint_max:
+lemma undefined_lit_count_decided_uint_max: 
   assumes
     M_\<L>\<^sub>a\<^sub>l\<^sub>l: \<open>\<forall>L\<in>set M. lit_of L \<in># \<L>\<^sub>a\<^sub>l\<^sub>l\<close> and n_d: \<open>no_dup M\<close> and
     \<open>L \<in> snd ` D\<^sub>0\<close> and \<open>undefined_lit M L\<close>
@@ -621,7 +825,7 @@ lemma undefined_lit_count_decided_uint_max:
 proof -
   have dist_atm_M: \<open>distinct_mset {#atm_of (lit_of x). x \<in># mset M#}\<close>
     using n_d by (metis distinct_mset_mset_distinct mset_map no_dup_def)
-  have \<open>atm_of `# lit_of `# mset (Decided L # M) \<subseteq># remdups_mset (atm_of `# \<L>\<^sub>a\<^sub>l\<^sub>l)\<close>
+  have incl: \<open>atm_of `# lit_of `# mset (Decided L # M) \<subseteq># remdups_mset (atm_of `# \<L>\<^sub>a\<^sub>l\<^sub>l)\<close>
     apply (subst distinct_subseteq_iff[THEN iffD1])
     using assms dist_atm_M
     by (auto simp: Decided_Propagated_in_iff_in_lits_of_l lits_of_def no_dup_distinct
@@ -647,6 +851,47 @@ proof -
 
   show ?thesis
     using 1 2 by (auto simp: uint_max_def)
+
+  from size_mset_mono[OF incl] have 1: \<open>length M + 1 \<le> size (remdups_mset (atm_of `# \<L>\<^sub>a\<^sub>l\<^sub>l))\<close>
+    unfolding uint_max_def count_decided_def
+    by (auto simp del: length_filter_le)
+  with 2 have \<open>length M  \<le> uint32_max\<close>
+    by auto
+qed
+
+lemma length_trail_uint_max:
+  assumes
+    M_\<L>\<^sub>a\<^sub>l\<^sub>l: \<open>\<forall>L\<in>set M. lit_of L \<in># \<L>\<^sub>a\<^sub>l\<^sub>l\<close> and n_d: \<open>no_dup M\<close>
+  shows \<open>length M \<le> uint_max\<close>
+proof -
+  have dist_atm_M: \<open>distinct_mset {#atm_of (lit_of x). x \<in># mset M#}\<close>
+    using n_d by (metis distinct_mset_mset_distinct mset_map no_dup_def)
+  have incl: \<open>atm_of `# lit_of `# mset M \<subseteq># remdups_mset (atm_of `# \<L>\<^sub>a\<^sub>l\<^sub>l)\<close>
+    apply (subst distinct_subseteq_iff[THEN iffD1])
+    using assms dist_atm_M
+    by (auto simp: Decided_Propagated_in_iff_in_lits_of_l lits_of_def no_dup_distinct
+        atm_of_eq_atm_of)
+
+  have inj_on: \<open>inj_on nat_of_lit (set_mset (remdups_mset \<L>\<^sub>a\<^sub>l\<^sub>l))\<close>
+    by (auto simp: inj_on_def)
+  have H: \<open>xa \<in># \<L>\<^sub>a\<^sub>l\<^sub>l \<Longrightarrow> atm_of xa \<le> uint_max div 2\<close> for xa
+    using in_\<L>\<^sub>a\<^sub>l\<^sub>l_less_uint_max
+    by (cases xa) (auto simp: uint_max_def)
+  have \<open>remdups_mset (atm_of `# \<L>\<^sub>a\<^sub>l\<^sub>l) \<subseteq># mset [0..< 1 + (uint_max div 2)]\<close>
+    apply (subst distinct_subseteq_iff[THEN iffD1])
+    using H distinct_image_mset_inj[OF inj_on]
+    by (force simp del: literal_of_nat.simps simp: distinct_mset_mset_set
+        dest: le_neq_implies_less)+
+  note _ = size_mset_mono[OF this]
+  moreover have \<open>size (nat_of_lit `# remdups_mset \<L>\<^sub>a\<^sub>l\<^sub>l) = size (remdups_mset \<L>\<^sub>a\<^sub>l\<^sub>l)\<close>
+    by simp
+  ultimately have 2: \<open>size (remdups_mset (atm_of `# \<L>\<^sub>a\<^sub>l\<^sub>l)) \<le> 1 + uint_max div 2\<close>
+    by auto
+  from size_mset_mono[OF incl] have 1: \<open>length M \<le> size (remdups_mset (atm_of `# \<L>\<^sub>a\<^sub>l\<^sub>l))\<close>
+    unfolding uint_max_def count_decided_def
+    by (auto simp del: length_filter_le)
+  with 2 show ?thesis
+    by (auto simp: uint32_max_def)
 qed
 
 definition (in -) get_pol where
@@ -894,19 +1139,20 @@ proof -
 qed
 
 definition (in isasat_input_ops) tl_trailt_tr :: \<open>trail_pol \<Rightarrow> trail_pol\<close> where
-  \<open>tl_trailt_tr = (\<lambda>(M', xs, lvls, reasons, k). 
+  \<open>tl_trailt_tr = (\<lambda>(M', xs, lvls, reasons, k, cs). 
     let L = last M' in
     (butlast M',
     let xs = xs[nat_of_lit L := None] in xs[nat_of_lit (-L) := None],
     lvls[atm_of L := zero_uint32_nat],
-    reasons, if reasons ! atm_of L = None then k-one_uint32_nat else k))\<close>
+    reasons, if reasons ! atm_of L = None then k-one_uint32_nat else k,
+      if reasons ! atm_of L = None then butlast cs else cs))\<close>
 
 sepref_thm tl_trail_tr_code
   is \<open>RETURN o tl_trailt_tr\<close>
-  :: \<open>[\<lambda>(M, xs, lvls, reason, k). M \<noteq> [] \<and> nat_of_lit(last M) < length xs \<and>
+  :: \<open>[\<lambda>(M, xs, lvls, reason, k, cs). M \<noteq> [] \<and> nat_of_lit(last M) < length xs \<and>
         nat_of_lit(-last M) < length xs  \<and> atm_of (last M) < length lvls \<and>
         atm_of (last M) < length reason \<and>
-    (reason ! atm_of (last M) = None \<longrightarrow> k \<ge> 1)]\<^sub>a
+        (reason ! atm_of (last M) = None \<longrightarrow> k \<ge> 1 \<and> cs \<noteq> [])]\<^sub>a
         trail_pol_assn\<^sup>d \<rightarrow> trail_pol_assn\<close>
   supply if_splits[split] option.splits[split]
   unfolding tl_trailt_tr_def UNSET_def[symmetric]
@@ -926,10 +1172,10 @@ lemmas tl_trail_tr_coded_refine[sepref_fr_rules] =
 
 sepref_thm tl_trail_tr_fast_code
   is \<open>RETURN o tl_trailt_tr\<close>
-  :: \<open>[\<lambda>(M, xs, lvls, reason, k). M \<noteq> [] \<and> nat_of_lit(last M) < length xs \<and>
+  :: \<open>[\<lambda>(M, xs, lvls, reason, k, cs). M \<noteq> [] \<and> nat_of_lit(last M) < length xs \<and>
         nat_of_lit(-last M) < length xs  \<and> atm_of (last M) < length lvls \<and>
         atm_of (last M) < length reason \<and>
-    (reason ! atm_of (last M) = None \<longrightarrow> k \<ge> 1)]\<^sub>a
+    (reason ! atm_of (last M) = None \<longrightarrow> k \<ge> 1 \<and> cs \<noteq> [])]\<^sub>a
         trail_pol_fast_assn\<^sup>d \<rightarrow> trail_pol_fast_assn\<close>
   supply if_splits[split] option.splits[split]
   unfolding tl_trailt_tr_def UNSET_def[symmetric]
@@ -949,6 +1195,9 @@ lemmas tl_trail_tr_fast_coded_refine[sepref_fr_rules] =
 lemma (in isasat_input_ops) ann_lits_split_reasons_map_lit_of:
   \<open>((M, reasons), M') \<in> ann_lits_split_reasons \<Longrightarrow>  M = map lit_of (rev M')\<close>
   by (auto simp: ann_lits_split_reasons_def)
+
+lemma control_stack_dec_butlast: \<open>control_stack b (Decided x1 # M's) \<Longrightarrow> control_stack (butlast b) M's\<close>
+  by (cases b rule: rev_cases) (auto dest: control_stackE)
 
 lemma tl_trail_tr:
   \<open>((RETURN o tl_trailt_tr), (RETURN o tl)) \<in>
@@ -984,6 +1233,11 @@ proof -
             dest: no_dup_consistentD)
       subgoal
         by (auto simp: tl_trailt_tr_def)
+      subgoal
+        by (cases \<open>L\<close>)
+          (auto simp: tl_trailt_tr_def in_\<L>\<^sub>a\<^sub>l\<^sub>l_atm_of_in_atms_of_iff ann_lits_split_reasons_def
+            control_stack_dec_butlast
+            dest: no_dup_consistentD)
       done
     done
 qed
@@ -1004,13 +1258,13 @@ proof -
     by (cases x rule: rev_cases) auto
   have H: \<open>?c
       \<in>  [comp_PRE trail_pol (\<lambda>M. M \<noteq> [])
-     (\<lambda>_ (M, xs, lvls, reason, k).
+     (\<lambda>_ (M, xs, lvls, reason, k, cs).
          M \<noteq> [] \<and>
          nat_of_lit (last M) < length xs \<and>
          nat_of_lit (-last M) < length xs \<and>
          atm_of (last M) < length lvls \<and>
          atm_of (last M) < length reason \<and>
-         (reason ! atm_of (last M) = None \<longrightarrow> 1 \<le> k))
+         (reason ! atm_of (last M) = None \<longrightarrow> 1 \<le> k \<and> cs \<noteq> []))
      (\<lambda>_. True)]\<^sub>a hrp_comp (trail_pol_assn\<^sup>d)
                     trail_pol \<rightarrow> hr_comp trail_pol_assn trail_pol\<close>
     (is \<open>_ \<in> [?pre']\<^sub>a ?im' \<rightarrow> ?f'\<close>)
@@ -1032,13 +1286,13 @@ proof -
     using pre ..
   have H: \<open>?cfast
       \<in>  [comp_PRE trail_pol (\<lambda>M. M \<noteq> [])
-     (\<lambda>_ (M, xs, lvls, reason, k).
+     (\<lambda>_ (M, xs, lvls, reason, k, cs).
          M \<noteq> [] \<and>
          nat_of_lit (last M) < length xs \<and>
          nat_of_lit (-last M) < length xs \<and>
          atm_of (last M) < length lvls \<and>
          atm_of (last M) < length reason \<and>
-         (reason ! atm_of (last M) = None \<longrightarrow> 1 \<le> k))
+         (reason ! atm_of (last M) = None \<longrightarrow> 1 \<le> k \<and> cs \<noteq> []))
      (\<lambda>_. True)]\<^sub>a hrp_comp (trail_pol_fast_assn\<^sup>d)
                     trail_pol \<rightarrow> hr_comp trail_pol_fast_assn trail_pol\<close>
     (is \<open>_ \<in> [?pre']\<^sub>a ?im' \<rightarrow> ?f'\<close>)
@@ -1135,9 +1389,10 @@ definition cons_trail_Decided :: \<open>nat literal \<Rightarrow> (nat, nat) ann
   \<open>cons_trail_Decided L M' = Decided L # M'\<close>
 
 definition cons_trail_Decided_tr :: \<open>nat literal \<Rightarrow> trail_pol \<Rightarrow> trail_pol\<close> where
-  \<open>cons_trail_Decided_tr = (\<lambda>L (M', xs, lvls, reasons, k).
+  \<open>cons_trail_Decided_tr = (\<lambda>L (M', xs, lvls, reasons, k, cs).
+    let n = length M' in
      (M' @ [L], let xs = xs[nat_of_lit L := Some True] in xs[nat_of_lit (-L) := Some False],
-      lvls[atm_of L := k+1], reasons[atm_of L := None], k+1))\<close>
+      lvls[atm_of L := k+1], reasons[atm_of L := None], k+1, cs @ [nat_of_uint32_spec n]))\<close>
 
 lemma cons_trail_Decided_tr:
   \<open>(uncurry (RETURN oo cons_trail_Decided_tr), uncurry (RETURN oo cons_trail_Decided)) \<in>
@@ -1147,13 +1402,14 @@ lemma cons_trail_Decided_tr:
         Decided_Propagated_in_iff_in_lits_of_l
         cons_trail_Decided_tr_def nth_list_update' ann_lits_split_reasons_def
       dest!: in_list_pos_neg_notD multi_member_split
+      intro: control_stack.cons_dec
       simp del: nat_of_lit.simps)
 
 sepref_thm cons_trail_Decided_tr_code
   is \<open>uncurry (RETURN oo cons_trail_Decided_tr)\<close>
-  :: \<open>[\<lambda>(L, (M, xs, lvls, reason, k)). nat_of_lit L < length xs \<and> nat_of_lit (-L) < length xs \<and>
+  :: \<open>[\<lambda>(L, (M, xs, lvls, reason, k, cs)). nat_of_lit L < length xs \<and> nat_of_lit (-L) < length xs \<and>
       atm_of L < length lvls \<and> atm_of L < length reason \<and> L \<in> snd ` D\<^sub>0 \<and>
-      Suc k \<le> uint_max]\<^sub>a
+      Suc k \<le> uint_max \<and> length M \<le> uint32_max]\<^sub>a
        unat_lit_assn\<^sup>k *\<^sub>a trail_pol_assn\<^sup>d \<rightarrow> trail_pol_assn\<close>
   unfolding cons_trail_Decided_tr_def cons_trail_Decided_tr_def one_uint32_nat_def[symmetric]
     get_pol_def[symmetric] SET_TRUE_def[symmetric] SET_FALSE_def[symmetric]
@@ -1172,9 +1428,9 @@ lemmas cons_trail_Decided_tr_code[sepref_fr_rules] =
 
 sepref_thm cons_trail_Decided_tr_fast_code
   is \<open>uncurry (RETURN oo cons_trail_Decided_tr)\<close>
-  :: \<open>[\<lambda>(L, (M, xs, lvls, reason, k)). nat_of_lit L < length xs \<and> nat_of_lit (-L) < length xs \<and>
+  :: \<open>[\<lambda>(L, (M, xs, lvls, reason, k, cs)). nat_of_lit L < length xs \<and> nat_of_lit (-L) < length xs \<and>
       atm_of L < length lvls \<and> atm_of L < length reason \<and> L \<in> snd ` D\<^sub>0 \<and>
-      Suc k \<le> uint_max]\<^sub>a
+      Suc k \<le> uint_max \<and> length M \<le> uint32_max]\<^sub>a
        unat_lit_assn\<^sup>k *\<^sub>a trail_pol_fast_assn\<^sup>d \<rightarrow> trail_pol_fast_assn\<close>
   unfolding cons_trail_Decided_tr_def cons_trail_Decided_tr_def one_uint32_nat_def[symmetric]
     get_pol_def[symmetric] SET_TRUE_def[symmetric] SET_FALSE_def[symmetric]
@@ -1204,11 +1460,11 @@ lemma
 proof -
   have H: \<open>?c \<in>  [comp_PRE (Id \<times>\<^sub>f trail_pol)
      (\<lambda>(L, M). undefined_lit M L \<and> L \<in> snd ` D\<^sub>0)
-     (\<lambda>_ (L, M, xs, lvls, reason, k).
+     (\<lambda>_ (L, M, xs, lvls, reason, k, cs).
          nat_of_lit L < length xs \<and>
          nat_of_lit (-L) < length xs \<and>
          atm_of L < length lvls \<and>
-         atm_of L < length reason \<and> L \<in> snd ` D\<^sub>0 \<and> Suc k \<le> uint_max)
+         atm_of L < length reason \<and> L \<in> snd ` D\<^sub>0 \<and> Suc k \<le> uint_max \<and> length M \<le> uint32_max)
      (\<lambda>_. True)]\<^sub>a hrp_comp (unat_lit_assn\<^sup>k *\<^sub>a trail_pol_assn\<^sup>d)
                     (Id \<times>\<^sub>f
                      trail_pol) \<rightarrow> hr_comp trail_pol_assn trail_pol\<close>
@@ -1217,7 +1473,7 @@ proof -
         OF isasat_input_bounded_axioms] .
   have pre: \<open>?pre' = ?pre\<close>
     by (auto simp: comp_PRE_def trail_pol_def image_image ann_lits_split_reasons_def uminus_\<A>\<^sub>i\<^sub>n_iff
-        intro!: ext undefined_lit_count_decided_uint_max)
+        intro!: ext undefined_lit_count_decided_uint_max length_trail_uint_max)
   have im: \<open>?im' = ?im\<close>
     unfolding prod_hrp_comp hrp_comp_dest hrp_comp_keep
     by (auto simp: hrp_comp_def hr_comp_def)
@@ -1228,11 +1484,11 @@ proof -
     using H unfolding im pre .
   have H: \<open>?cfast \<in>  [comp_PRE (Id \<times>\<^sub>f trail_pol)
      (\<lambda>(L, M). undefined_lit M L \<and> L \<in> snd ` D\<^sub>0)
-     (\<lambda>_ (L, M, xs, lvls, reason, k).
+     (\<lambda>_ (L, M, xs, lvls, reason, k, cs).
          nat_of_lit L < length xs \<and>
          nat_of_lit (-L) < length xs \<and>
          atm_of L < length lvls \<and>
-         atm_of L < length reason \<and> L \<in> snd ` D\<^sub>0 \<and> Suc k \<le> uint_max)
+         atm_of L < length reason \<and> L \<in> snd ` D\<^sub>0 \<and> Suc k \<le> uint_max \<and> length M \<le> uint32_max)
      (\<lambda>_. True)]\<^sub>a hrp_comp (unat_lit_assn\<^sup>k *\<^sub>a trail_pol_fast_assn\<^sup>d)
                     (Id \<times>\<^sub>f
                      trail_pol) \<rightarrow> hr_comp trail_pol_fast_assn trail_pol\<close>
